% SIAM Article Template
\documentclass[onecolumn,final,a4paper,13pt,reqno]{siamart}

% Information that is shared between the article and the supplement
% (title and author information, macros, packages, etc.) goes into
% ex_shared.tex. If there is no supplement, this file can be included
% directly.

% Packages and macros go here
\usepackage{lipsum}
\usepackage{amsfonts}
\usepackage{graphicx}
\usepackage{epstopdf}
\usepackage{algorithmic}
\usepackage{xspace}
\usepackage{enumitem}
\usepackage[font=small]{caption}
\usepackage{subcaption}
\usepackage{pgfplots}
\usepackage{tikz}
\usepackage[top=3cm,bottom=3cm,left=2.5cm,right=2.5cm]{geometry}

% http://tex.stackexchange.com/questions/36278/box-around-theorem-statement
% http://tex.stackexchange.com/questions/188051/skipbelow-does-not-work-for-combination-of-mdframed-and-thmtools
%\usepackage{amsthm}
\usepackage{thmtools}
\usepackage{mdframed}

\declaretheoremstyle[
	postfoothook={\vskip 0.35cm},
	mdframed={
		skipabove=0.35cm,
		innerbottommargin=0.2cm,
		innertopmargin=0.2cm,
		innerleftmargin=0.2cm,
		innerrightmargin=0.2cm,
	}
]{skips}

\declaretheorem[style=skips,name={Theorem}]{theoremmd}
\declaretheorem[style=skips,name={Corollary}]{corollarymd}
\declaretheorem[style=skips,name={Lemma}]{lemmamd}
\declaretheorem[style=skips,name={Definition}]{definitionmd}

% http://tex.stackexchange.com/questions/4728/how-do-i-number-equations-only-if-they-are-referred-to-in-the-text
%\usepackage{mathtools}
%\mathtoolsset{showonlyrefs=true}
\usepackage{autonum}

% http://tex.stackexchange.com/questions/8092/placing-equation-number-on-left-with-reqno-option-in-amsart-document-class
\usepackage{environ}
\makeatletter
\NewEnviron{Lalign}{\tagsleft@true\begin{align}\BODY\end{align}}
\makeatother

% http://tex.stackexchange.com/questions/23773/a-centered-plus-minus-symbol
\newcommand{\rpm}{\raisebox{.2ex}{$\scriptstyle\pm$}}

\ifpdf
  \DeclareGraphicsExtensions{.eps,.pdf,.png,.jpg}
\else
  \DeclareGraphicsExtensions{.eps}
\fi

\makeatletter
\DeclareRobustCommand\onedot{\futurelet\@let@token\@onedot}
\def\@onedot{\ifx\@let@token.\else.\null\fi\xspace}
\def\eg{{e.g}\onedot} \def\Eg{{E.g}\onedot}
\def\ie{{i.e}\onedot} \def\Ie{{I.e}\onedot}
\def\cf{{c.f}\onedot} \def\Cf{{C.f}\onedot}
\def\etc{{etc}\onedot} \def\vs{{vs}\onedot}
\def\wrt{w.r.t\onedot} \def\dof{d.o.f\onedot}
\def\etal{{et al}\onedot}

% proximal map operator
\DeclareRobustCommand{\prox}[1]{%
    \ifmmode
        \text{prox}_{#1}
    \else
        $\text{prox}_{#1}$
    \fi
}
\def\dom{\text{dom}}
\def\per{\text{per}}

% Declare title and authors, without \thanks
\newcommand{\TheTitle}{iPiano: Inertial Proximal Algorithm for Non-Convex Optimization} 
\newcommand{\TheAuthors}{D. Stutz}

% Sets running headers as well as PDF title and authors
\headers{\TheTitle}{\TheAuthors}

% Title. If the supplement option is on, then "Supplementary Material"
% is automatically inserted before the title.
\title{{\TheTitle}}

% Authors: full names plus addresses.
\author{
  David Stutz\thanks{Submitted as part of the seminar "Ausgew\"ahlte Themen der Bildverarbeitung'', WS 2015/2016, and advised by Prof. Berkels, AICES, RWTH Aachen University.}
}

\usepackage{amsopn}
\DeclareMathOperator{\diag}{diag}

% Optional PDF information
\ifpdf
\hypersetup{
  pdftitle={\TheTitle},
  pdfauthor={\TheAuthors}
}
\fi

\begin{document}
	\maketitle
	
	Composite function:
	\begin{align}
		\min_{x \in \mathbb{R}^n} h(x) = \min_{x \in \mathbb{R}^n} (\underbrace{f(x)}_{\begin{tabular}{c}$\in C^1$\\$\nabla f$ Lipschitz-continuous\end{tabular}} + \underbrace{g(x)}_{\begin{tabular}{l}proper closed convex\\lower semicontinuous\end{tabular}})
	\end{align}
	with
	\begin{align}
		-\infty < h_{\min} := \inf _{x \in \mathbb{R}^n} h(x)
	\end{align}
	\noindent\rule{\textwidth}{0.1pt}
	
	Iteration:
	\begin{align}
		x^{(n + 1)} = \prox{\alpha_n g}(x^{(n)} - \alpha_n \nabla f(x^{(n)}) + \beta_n(x^{(n)} - x^{(n - 1)})).\label{eq:iteration}
	\end{align}
	\noindent\rule{\textwidth}{0.1pt}
	
	Backtracking:
	\begin{align}
		f(x^{(n + 1)}) \leq f(x^{(n)}) + &\nabla f(x^{(n)})^T (x^{(n + 1)} - x^{(n)}) + \frac{L_n}{2} \|x^{(n + 1)} - x^{(n)}\|_2^2
	\end{align}
	\noindent\rule{\textwidth}{0.1pt}
	
	Remember:
	\begin{align}
		\delta_n := \frac{1}{\alpha_n} - \frac{L_n}{2} - \frac{\beta_n}{2\alpha_n} \geq \gamma_n\label{eq:delta}\\
		\gamma_n := \frac{1}{\alpha_n} - \frac{L_n}{2} - \frac{\beta_n}{\alpha_n} \geq c_2\label{eq:gamma}
	\end{align}
	\noindent\rule{\textwidth}{0.1pt}
	
	\textbf{Proof Sketch (Monotonicity)}\\
	Using \eqref{eq:delta} and \eqref{eq:gamma}
	\begin{align}
		\gamma_n \geq c_2 \quad\Leftrightarrow\quad \alpha_n \leq \frac{1 - \beta_n}{c_2 + \frac{L_n}{2}} < \frac{2(1 - \beta_n)}{L_n}\label{eq:alpha}
	\end{align}
	To show monotonicity of $\delta_n$:
	\begin{align}
		\delta_{n - 1} &\geq \delta_n := \frac{1}{\alpha_n} - \frac{L_n}{2} - \frac{\beta_n}{2\alpha_n}\quad\Leftrightarrow\quad \alpha_n \geq \frac{1 - \frac{\beta_n}{2}}{\delta_{n - 1} + \frac{L_n}{2}};
	\end{align}
	with \eqref{eq:alpha}:
	\begin{align}
		\delta_{n - 1} &\geq \delta_n \text{ }\Leftrightarrow\text{ } \frac{1 - \beta_n}{c_2 + \frac{L_n}{2}} \geq \alpha_n \geq \frac{1 - \frac{\beta_n}{2}}{\delta_{n - 1} + \frac{L_n}{2}}\text{ }\Rightarrow\text{ } \beta_n \leq \frac{b_n - 1}{b_n - \frac{1}{2}}
	\end{align}
	with $b_n := (\delta_{n - 1} + \frac{L_n}{2})/(c_2 + \frac{L_n}{2})$.

	\noindent\rule{\textwidth}{0.1pt}
	
	Remember:
	\begin{align}
		H_{\delta_{n + 1}}(x^{(n + 1)}, x^{(n)}) := h(x^{(n + 1)}) + \delta_{n + 1}\Delta_{n + 1}^2
	\end{align}
	and
	\begin{align}
		(z^{(n + 1)})_{n \in \mathbb{N}} = (x^{(n + 1)}, x^{(n)})_{n \in \mathbb{N}}.
	\end{align}
	
	\textbf{Proof Sketch (Condition (H1))}\\
	From \eqref{eq:iteration}:
	\begin{align}
		w:= \frac{x^{(n)} - x^{(n + 1)}}{\alpha_n} - \nabla f(x^{(n)}) + \frac{\beta_n}{\alpha_n} (x^{(n)} - x^{(n - 1)}) \in \partial g(x^{(n + 1)}) \label{eq:subdifferential}
	\end{align}
	With
	\begin{align}
		g(x^{(n + 1)}) \overset{convex}{\leq} g(x^{(n)}) - w^T(x^{(n)} - x^{(n - 1)})
	\end{align}
	and
	\begin{align}
		f(x^{(n + 1)}) \leq f(x^{(n)}) - + \nabla f(x^{(n)})^T(x^{(n + 1)} - x^{(n)}) + \frac{L_n}{2}\|x^{(n)} - x^{(n + 1)}\|_2^2
	\end{align}
	the claim follows from
	\begin{align}
		h(x^{(n + 1)}) \leq h(x^{(n)}) - \delta_n\Delta_{n + 1}^2 + \delta_n\Delta_n^2 - \gamma_n \Delta_n^2.
	\end{align}
	\noindent\rule{\textwidth}{0.1pt}
	
	\textbf{Proof Sketch (Condition (H2))}\\
	For $w^{(n + 1)} \in \partial H_{\delta_{n + 1}}(z^{(n + 1)})$ it is $w^{(n + 1)} = (w_1^{(n + 1)}, w_2^{(n + 1)})$ with
	\begin{align}
		w_1^{(n + 1)} &\in \partial g(x^{(n + 1)}) + \nabla f(x^{(n + 1)}) + 2 \delta_n (x^{(n + 1)} - x^{(n)})\\
		w_2^{(n + 1)} &= -2\delta_n(x^{(n + 1)} - x^{(n)})
	\end{align}
	and with Equation \eqref{eq:subdifferential}
	\begin{align}
		\|w^{(n + 1)}\|_2 \leq ... \leq (\frac{1}{\alpha_n} + 4\delta_n + L_n)\Delta_{n + 1} + \frac{\beta_n}{\alpha_n} \Delta_n \leq \frac{7}{c_1}(\Delta_{n + 1} + \Delta_n)
	\end{align}
	\noindent\rule{\textwidth}{0.1pt}
	
	\textbf{Proof Sketch (Condition (H3))}\\
	Remember: 
	\begin{Lalign}
		H_{\delta_{n + 1}}(z^{(n + 1)}) + \gamma_n\Delta_n^2 \leq H_{\delta_n}(z^{(n)})\label{cond:1}\tag{H1}.
	\end{Lalign}
	Claim 1: $\lim_{n \rightarrow \infty} \Delta_n = 0$\\
	Summing Condition \eqref{cond:1} and deducing $\sum_{n = 0}^\infty \Delta_n^2 < \infty$ it follows $\lim_{n \rightarrow \infty} \Delta_n = 0$.
	
	Claim 2: it exists a subsequence $(x^{(n_j)})_{j \in \mathbb{N}}$ with $\tilde{x} = \lim_{j \rightarrow \infty} x^{(n_j)}$.\\
	The convergence of $h(x^{(n)})$ follows from the squeeze theorem:
	\begin{align}
		H_{-\delta_n}(x^{(n)}, x^{(n - 1)}) \leq h(x^{(n)}) \leq H_{\delta_n}(x^{(n)}, x^{(n - 1)})
	\end{align}
	as $H(x^{(n)}, x^{(n - 1)})$ converges (monotonically decreasing and $h$ bounded below).
	From the coercivity of $h$ and the Bolzano-Weierstrass theorem the existence of the subsequence follows.
	
	Then:
	\begin{align}
		\lim_{j \rightarrow \infty} H_{\delta_{n_j + 1}}(x^{(n_j + 1)}, x^{(n_j)}) = \lim_{j \rightarrow \infty} h(x^{(n_j + 1)}) + \underbrace{\delta_n\|x^{(n_j + 1)} - x^{(n_j)}\|_2}_{\rightarrow 0} = H_\delta(\tilde{x}, \tilde{x}) = h(\tilde{x}).
	\end{align}
	\noindent\rule{\textwidth}{0.1pt}
	
	\textbf{Proof Sketch (Theorem)}\\
	Remember: it exists $w^{(n)} \in \partial H(z^{(n)})$ such that
	\begin{Lalign}
		\|w^{(n)}\|_2 \leq \frac{b}{2}(\Delta_n + \Delta_{n - 1})\label{cond:2}\tag{H2}.
	\end{Lalign}
	The proof is based on the following claim:
	\begin{align}
		\sum_{i = 1}^n \Delta_i \leq \frac{1}{2}(\Delta_0 - \Delta_n) + \frac{b}{a}\left[\phi(H(z^{(1)}) - H(\tilde{z})) - \phi(H(z^{(n + 1)}) - H(\tilde{z}))\right]
	\end{align}
	which is shown by induction. Then, it follows $\sum_{n = 0}^\infty \Delta_n < \infty$ and $x^{(n)} \rightarrow \tilde{x}$. Using the Kurdyka-Lojasiewicz property it can be shown that $H_{\delta_n}(z^{(n)}) \rightarrow H(\tilde{z})$. With Condition \eqref{cond:2} it also follows that $\tilde{z}$ is a critical point of $H$.
	
\end{document}
